compiler/backend/semantics/bviPropsScript.sml
@@ -64,24 +64,21 @@ val list_thms = { nchotomy = list_nchotomy, case_def = list_case_def };
 val option_thms = { nchotomy = option_nchotomy, case_def = option_case_def };
 val result_thms = { nchotomy = semanticPrimitivesTheory.result_nchotomy,
                     case_def = semanticPrimitivesTheory.result_case_def };
-val op_thms = { nchotomy = closLangTheory.op_nchotomy, case_def = closLangTheory.op_case_def };
-val v_thms = { nchotomy = bvlSemTheory.v_nchotomy, case_def = bvlSemTheory.v_case_def };
-val ref_thms = { nchotomy = closSemTheory.ref_nchotomy, case_def = closSemTheory.ref_case_def };
-val eq_result_thms = { nchotomy = semanticPrimitivesTheory.eq_result_nchotomy,
-                       case_def = semanticPrimitivesTheory.eq_result_case_def };
-val word_size_thms = { nchotomy = astTheory.word_size_nchotomy,
-                       case_def = astTheory.word_size_case_def };
 
 val pair_case_elim = prove(
   ``pair_CASE p f ⇔ ∃x y. p = (x,y) ∧ f x y``,
   Cases_on`p` \\ rw[]);
 
 val elims = List.map prove_case_elim_thm [
-  list_thms, result_thms ] |> cons pair_case_elim |> LIST_CONJ;
+  list_thms, option_thms, result_thms ] |> cons pair_case_elim |> LIST_CONJ
+  |> curry save_thm "case_elim_thms";
+val case_elim_thms = elims;
 
-val case_eq_thms = List.map prove_case_eq_thm [
-  list_thms, option_thms, result_thms, op_thms, v_thms,
-  ref_thms, eq_result_thms, word_size_thms ] |> LIST_CONJ;
+val case_eq_thms =
+  CONJ
+  (prove_case_eq_thm {nchotomy = bviTheory.exp_nchotomy, case_def = bviTheory.exp_case_def})
+  bvlPropsTheory.case_eq_thms
+  |> curry save_thm "case_eq_thms";
 
 val evaluate_LENGTH = Q.prove(
   `!xs s env. (\(xs,s,env).
